GeneralLogic/ModelClass.v
@@ -1,0 +1,70 @@
+Require Import Coq.Classes.Morphisms.
+Require Import Logic.lib.Ensembles_ext.
+Require Import Logic.GeneralLogic.Base.
+
+Instance proper_strongly_complete
+         {L: Language}
+         {GammaD: Derivable L}
+         {MD: Model}
+         {SM: Semantics L MD}:
+  Proper (Same_set _ ==> iff) (strongly_complete GammaD SM).
+Proof.
+  hnf; intros MC1 MC2 ?.
+  unfold strongly_complete.
+  apply Morphisms_Prop.all_iff_morphism.
+  intro Phi.
+  apply Morphisms_Prop.all_iff_morphism.
+  intro x.
+  apply Morphisms_Prop.iff_iff_iff_impl_morphism; [| reflexivity].
+  unfold consequence.
+  rewrite Same_set_spec in H; hnf in H.
+  firstorder.
+Qed.
+
+Instance proper_weakly_complete
+         {L: Language}
+         {GammaP: Provable L}
+         {MD: Model}
+         {SM: Semantics L MD}:
+  Proper (Same_set _ ==> iff) (weakly_complete GammaP SM).
+Proof.
+  hnf; intros MC1 MC2 ?.
+  unfold weakly_complete.
+  apply Morphisms_Prop.all_iff_morphism.
+  intro x.
+  apply Morphisms_Prop.iff_iff_iff_impl_morphism; [| reflexivity].
+  unfold valid.
+  rewrite Same_set_spec in H; hnf in H.
+  firstorder.
+Qed.
+
+Instance proper_KripkeModelClass
+         {MD: Model}
+         {kMD: KripkeModel MD}:
+  Proper (Same_set _ ==> Same_set _) (KripkeModelClass MD).
+Proof.
+  hnf; intros.
+  rewrite Same_set_spec in H |- *.
+  hnf in H |- *.
+  intros; split; intros; inversion H0; constructor; subst; firstorder.
+Qed.
+
+Lemma KripkeModelClass_ModelClass_Same_set_spec
+      {MD: Model}
+      {kMD: KripkeModel MD}:
+  forall MC kMC,
+    (forall m: model, MC m <-> exists M w, kMC M /\ m = build_model M w) ->
+    Same_set _ MC (KripkeModelClass _ kMC).
+Proof.
+  intros.
+  rewrite Same_set_spec.
+  hnf; intros m; split; intros.
+  + rewrite H in H0.
+    destruct H0 as [M [w [? ?]]].
+    subst m.
+    constructor.
+    auto.
+  + inversion H0; subst.
+    rewrite H.
+    eauto.
+Qed.
